Cleanup of trace modifies analysis (Still has examples)

src/core/DY.Core.Trace.Modifies.fst
@@ -16,226 +16,245 @@ type modifies_set = set address
 
 /// Set lemmas
 
-let union_empty (#a:eqtype) (s:set a)
-  : Lemma (ensures union s empty == s /\ union empty s == s)
-    [SMTPatOr [
-      [SMTPat (union s empty)];
-      [SMTPat (union empty s)]
-    ]]
-  = assert(equal (union s empty) s); assert(equal (union empty s) s)
+val lemma_union_empty :
+  #a:eqtype -> s:set a ->
+  Lemma (union s empty == s /\ union empty s == s)
+  [SMTPatOr [
+    [SMTPat (union s empty)];
+    [SMTPat (union empty s)]
+  ]]
+let lemma_union_empty s =
+  assert(equal (union s empty) s);
+  assert(equal (union empty s) s)
 
-let union_add (#a:eqtype) (x:a) (s1 s2:set a)
-  : Lemma (ensures add x (union s1 s2) == union (add x s1) s2)
-  = assert(equal (add x (union s1 s2)) (union (add x s1) s2))
+// TODO: The next three lemmas may be unneeded here
+val lemma_add_is_union_singleton :
+  #a:eqtype -> x:a ->
+  s:set a ->
+  Lemma (add x s == union (singleton x) s)
+let lemma_add_is_union_singleton x s =
+  assert(equal (add x s) (union (singleton x) s))
 
-let union_assoc (#a:eqtype) (s1 s2 s3:set a)
-  : Lemma (ensures (union (union s1 s2) s3) == (union s1 (union s2 s3)))
-  = assert(equal (union (union s1 s2) s3) (union s1 (union s2 s3)))
+val lemma_union_assoc :
+  #a:eqtype ->
+  s1:set a -> s2:set a -> s3:set a ->
+  Lemma (union (union s1 s2) s3 == union s1 (union s2 s3))
+let lemma_union_assoc s1 s2 s3 =
+  assert(equal (union (union s1 s2) s3) (union s1 (union s2 s3)))
+
+val lemma_union_comm :
+  #a:eqtype ->
+  s1:set a -> s2:set a ->
+  Lemma (union s1 s2 == union s2 s1)
+let lemma_union_comm s1 s2 =
+  assert(equal (union s1 s2) (union s2 s1))
 
 /// Modifies functions
 
-let rec trace_modifies (#label_t:Type) (tr:trace_ label_t) : modifies_set
-  = match tr with
-    | Nil -> Set.empty
-    | Snoc hd (SetState p sid _) -> Set.add (p, sid) (trace_modifies hd)
-    | Snoc hd _ -> trace_modifies hd
+val trace_modifies :
+  #label_t:Type -> trace_ label_t ->
+  modifies_set
+let rec trace_modifies tr =
+  match tr with
+  | Nil -> Set.empty
+  | Snoc hd (SetState p sid _) -> Set.add (p, sid) (trace_modifies hd)
+  | Snoc hd _ -> trace_modifies hd
 
-let rec trace_modifies_spec (#label_t:Type) (tr:trace_ label_t) (prin:principal) (sid:state_id)
-  : Lemma
-    (ensures (
-      let mod_set = trace_modifies tr in
-      if Set.mem (prin, sid) mod_set
-      then exists b. state_was_set tr prin sid b
-      else forall b. ~(state_was_set tr prin sid b)
-    ))
-  = match tr with
-    | Nil -> ()
-    | Snoc hd (SetState prin' sid' b) -> begin
-      if prin' = prin && sid' = sid then ()
-      else trace_modifies_spec hd prin sid
-    end
-    | Snoc hd _ -> trace_modifies_spec hd prin sid
+val trace_modifies_spec :
+  #label_t:Type -> tr:trace_ label_t -> prin:principal -> sid:state_id ->
+  Lemma ((prin, sid) `mem` (trace_modifies tr) <==> exists b. state_was_set tr prin sid b)
+let rec trace_modifies_spec tr prin sid =
+  match tr with
+  | Nil -> ()
+  | Snoc hd (SetState prin' sid' b) -> begin
+    if prin' = prin && sid' = sid then ()
+    else trace_modifies_spec hd prin sid
+  end
+  | Snoc hd _ -> trace_modifies_spec hd prin sid
 
-let rec trace_modifies_concat (#label_t:Type) (tr1 tr2:trace_ label_t)
-  : Lemma
-    (ensures
-      trace_modifies (tr1 <++> tr2) == union (trace_modifies tr1) (trace_modifies tr2)
-    )
-    [SMTPat (trace_modifies (tr1 <++> tr2))]
-  = if is_empty tr2 then trace_concat_empty_trace tr1
-    else begin
-      trace_modifies_concat tr1 (init tr2);
-      trace_concat_append_entry tr1 (init tr2) (last tr2);
-      assert(equal (trace_modifies (tr1 <++> tr2)) (union (trace_modifies tr1) (trace_modifies tr2)))
-    end
-    // TODO: Can we get some of these lemmas to trigger more automatically?
-    // Additionally, can we find a way to remove the assertion here?
+val trace_modifies_concat  :
+  #label_t:Type ->
+  tr1:trace_ label_t -> tr2:trace_ label_t ->
+  Lemma (trace_modifies (tr1 <++> tr2) == union (trace_modifies tr1) (trace_modifies tr2))
+  [SMTPat (trace_modifies (tr1 <++> tr2))]
+let rec trace_modifies_concat tr1 tr2 =
+  if is_empty tr2 then trace_concat_empty_trace tr1
+  else begin
+    trace_modifies_concat tr1 (init tr2);
+    trace_concat_append_entry tr1 (init tr2) (last tr2);
+    // triggers lemma_equal_elim and lemma_equal_intro
+    assert(equal (trace_modifies (tr1 <++> tr2)) (union (trace_modifies tr1) (trace_modifies tr2)))
+  end
 
-let traceful_modifies (#a:Type) (f:traceful a) (tr_in:trace) : modifies_set
-  = let (_, tr_out) = f tr_in in
-    trace_modifies (tr_out <--> tr_in)
+val traceful_modifies :
+  #a:Type -> traceful a -> trace ->
+  modifies_set
+let traceful_modifies f tr_in =
+  let (_, tr_out) = f tr_in in
+  trace_modifies (tr_out <--> tr_in)
+
 
 /// Lemmas to automate modifies analysis
 
-let traceful_modifies_bind
-  (#a #b:Type)
-  (x:traceful a) (f:(a -> traceful b))
-  (tr_in:trace)
-  : Lemma
-    (requires True)
-    (ensures (
-      let bind_mod = traceful_modifies (let* x in f x) tr_in in
-      let x_mod = traceful_modifies x tr_in in
-      let (y, tr_mid) = x tr_in in
-      let f_mod = traceful_modifies (f y) tr_mid in
-      bind_mod == union x_mod f_mod
-    ))
-  = let (y, tr_mid) = x tr_in in
-    let (_, tr_out) = f y tr_mid in
-//    assert(tr_in <$ tr_mid /\ tr_mid <$ tr_out);
-    // Triggers trace_subtract_concat_slices
-    assert(((tr_mid <--> tr_in) <++> (tr_out <--> tr_mid)) == (tr_out <--> tr_in));
-//    assert(traceful_modifies x tr_in == trace_modifies (tr_mid <--> tr_in));
-//    assert(traceful_modifies (f y) tr_mid == trace_modifies (tr_out <--> tr_mid));
-//    assert(traceful_modifies (let* x in f x) tr_in == trace_modifies (tr_out <--> tr_in));
-//    admit();
-    ()
+val traceful_modifies_bind :
+  #a:Type -> #b:Type ->
+  x:traceful a -> f:(a -> traceful b) ->
+  tr_in:trace ->
+  Lemma
+  (ensures (
+    let (y, tr_mid) = x tr_in in
+    traceful_modifies ((let*) x f) tr_in ==
+    union (traceful_modifies x tr_in) (traceful_modifies (f y) tr_mid)
+  ))
+  [SMTPat (traceful_modifies ((let*) x f) tr_in)]
+let traceful_modifies_bind x f tr_in =
+  let (y, tr_mid) = x tr_in in
+  let (_, tr_out) = f y tr_mid in
+  // Triggers trace_subtract_concat_slices
+  assert(((tr_mid <--> tr_in) <++> (tr_out <--> tr_mid)) == (tr_out <--> tr_in))
 
-let traceful_modifies_return
-  (#a:Type) (x:a)
-  (tr:trace)
-  : Lemma
-    (ensures (
-      traceful_modifies (return x) tr == empty
-    ))
-    [SMTPat (traceful_modifies (return x) tr)]
-  = ()
+val traceful_modifies_return :
+  #a:Type ->
+  x:a -> tr:trace ->
+  Lemma (traceful_modifies (return x) tr == empty)
+  [SMTPat (traceful_modifies (return x) tr)]
+let traceful_modifies_return x tr = ()
 
-let traceful_modifies_get_trace (tr:trace)
-  : Lemma (ensures traceful_modifies get_trace tr == empty)
-    [SMTPat (traceful_modifies get_trace tr)]
-  = ()
+val traceful_modifies_get_trace :
+  tr:trace ->
+  Lemma (traceful_modifies get_trace tr == empty)
+  [SMTPat (traceful_modifies get_trace tr)]
+let traceful_modifies_get_trace tr = ()
 
-let traceful_modifies_guard_tr (b:bool) (tr:trace)
-  : Lemma (ensures (traceful_modifies (guard_tr b) tr) == empty)
-    [SMTPat (traceful_modifies (guard_tr b) tr)]
-  = ()
+val traceful_modifies_guard_tr :
+  b:bool -> tr:trace ->
+  Lemma (traceful_modifies (guard_tr b) tr == empty)
+  [SMTPat (traceful_modifies (guard_tr b) tr)]
+let traceful_modifies_guard_tr b tr = ()
 
-let traceful_modifies_add_entry_forall (e:trace_entry)
-  : Lemma
-    (ensures forall (tr:trace). (
-      traceful_modifies (add_entry e) tr ==
-      (match e with
-      | SetState prin sid _ -> singleton (prin, sid)
-      | _ -> empty
-      )
-    ))
-    [SMTPat (traceful_modifies (add_entry e))]
-  = assert(forall (tr:trace). add_entry e tr == ((), append_entry tr e))
+val traceful_modifies_add_entry :
+  e:trace_entry ->
+  tr:trace ->
+  Lemma
+  (ensures (
+    traceful_modifies (add_entry e) tr == (match e with
+    | SetState prin sid _ -> singleton (prin, sid)
+    | _ -> empty
+    )
+  ))
+  [SMTPat (traceful_modifies (add_entry e) tr)]
+let traceful_modifies_add_entry e tr =
+  /// TODO Can we find a way to remove the need for these next two lines?
+  let (_, tr_out) = add_entry e tr in
+  assert(tr_out == append_entry tr e);
+  match e with
+  | SetState prin sid _ -> assert(equal (add (prin, sid) empty) (singleton (prin, sid)))
+  | _ -> ()
 
-let traceful_modifies_add_entry
-  (e:trace_entry)
-  (tr:trace)
-  : Lemma
-    (ensures (
-      match e with
-      | SetState prin sid _ -> traceful_modifies (add_entry e) tr == singleton (prin, sid)
-      | _ -> traceful_modifies (add_entry e) tr == empty
-    ))
-    [SMTPat (add_entry e tr)]
-  = match e with
-    | SetState prin sid _ -> begin
-      /// TODO Find a way to remove the need for these next two lines
-      let (_, tr_out) = add_entry e tr in
-      assert(tr_out == append_entry tr e);
-      assert(equal (add (prin, sid) empty) (singleton (prin, sid)))
-    end
-    | _ -> begin
-      let (_, tr_out) = add_entry e tr in
-      assert(tr_out == append_entry tr e);
-      ()
-    end
+val traceful_modifies_get_time :
+  tr:trace ->
+  Lemma (traceful_modifies get_time tr == empty)
+  [SMTPat (traceful_modifies get_time tr)]
+let traceful_modifies_get_time tr = ()
 
-let traceful_modifies_get_time (tr:trace)
-  : Lemma (ensures traceful_modifies get_time tr == empty)
-    [SMTPat (traceful_modifies get_time tr)]
-  = ()
+val traceful_modifies_send_msg :
+  b:bytes -> tr:trace ->
+  Lemma (traceful_modifies (send_msg b) tr == empty)
+  [SMTPat (traceful_modifies (send_msg b) tr)]
+let traceful_modifies_send_msg b tr =
+  reveal_opaque (`%send_msg) (send_msg)
 
-let traceful_modifies_send_msg (b:bytes) (tr:trace)
-  : Lemma (ensures traceful_modifies (send_msg b) tr == empty)
-    [SMTPat (traceful_modifies (send_msg b) tr)]
-  = reveal_opaque (`%send_msg) (send_msg);
-    // TODO: Can we remove the need for this assert?
-    assert(traceful_modifies (add_entry (MsgSent b)) tr == empty)
+val traceful_modifies_recv_msg :
+  ts:timestamp -> tr:trace ->
+  Lemma (traceful_modifies (recv_msg ts) tr == empty)
+  [SMTPat (traceful_modifies (recv_msg ts) tr)]
+let traceful_modifies_recv_msg ts tr = ()
 
-let traceful_modifies_recv_msg (ts:timestamp) (tr:trace)
-  : Lemma (ensures traceful_modifies (recv_msg ts) tr == empty)
-    [SMTPat (traceful_modifies (recv_msg ts) tr)]
-  = ()
+val traceful_modifies_mk_rand :
+  usg:usage -> lab:label -> len:nat{len <> 0} -> tr:trace ->
+  Lemma (traceful_modifies (mk_rand usg lab len) tr == empty)
+  [SMTPat (traceful_modifies (mk_rand usg lab len) tr)]
+let traceful_modifies_mk_rand usg lab len tr =
+  reveal_opaque (`%mk_rand) (mk_rand)
 
-let traceful_modifies_mk_rand (usg:usage) (lab:label) (len:nat{len <> 0}) (tr:trace)
-  : Lemma (ensures (traceful_modifies (mk_rand usg lab len) tr == empty))
-    [SMTPat (traceful_modifies (mk_rand usg lab len) tr)]
-  = reveal_opaque (`%mk_rand) (mk_rand)
+val traceful_modifies_set_state :
+  prin:principal -> sid:state_id -> b:bytes -> tr:trace ->
+  Lemma (traceful_modifies (set_state prin sid b) tr == singleton (prin, sid))
+  [SMTPat (traceful_modifies (set_state prin sid b) tr)]
+let traceful_modifies_set_state prin sid b tr =
+  reveal_opaque (`%set_state) (set_state)
 
-let traceful_modifies_set_state (prin:principal) (sid:state_id) (b:bytes) (tr:trace)
-  : Lemma (ensures (traceful_modifies (set_state prin sid b) tr == singleton (prin, sid)))
-    [SMTPat (traceful_modifies (set_state prin sid b) tr)]
-   = reveal_opaque (`%set_state) (set_state)
+val traceful_modifies_new_session_id :
+  prin:principal -> tr:trace ->
+  Lemma (traceful_modifies (new_session_id prin) tr == empty)
+  [SMTPat (traceful_modifies (new_session_id prin) tr)]
+let traceful_modifies_new_session_id prin tr = ()
 
-let traceful_modifies_new_session_id (prin:principal) (tr:trace)
-  : Lemma (ensures (traceful_modifies (new_session_id prin) tr) == empty)
-   [SMTPat (traceful_modifies (new_session_id prin) tr)]
-  = ()
+val traceful_modifies_get_state :
+  prin:principal -> sid:state_id -> tr:trace ->
+  Lemma (traceful_modifies (get_state prin sid) tr == empty)
+  [SMTPat (traceful_modifies (get_state prin sid) tr)]
+let traceful_modifies_get_state prin sid tr = ()
 
-let traceful_modifies_get_state (prin:principal) (sid:state_id) (tr:trace)
-  : Lemma (ensures (traceful_modifies (get_state prin sid) tr) == empty)
-    [SMTPat (traceful_modifies (get_state prin sid) tr)]
-  = ()
+val traceful_modifies_trigger_event :
+  prin:principal -> tag:string -> b:bytes -> tr:trace ->
+  Lemma (traceful_modifies (trigger_event prin tag b) tr == empty)
+  [SMTPat (traceful_modifies (trigger_event prin tag b) tr)]
+let traceful_modifies_trigger_event prin tag b tr =
+  reveal_opaque (`%trigger_event) (trigger_event)
 
-let traceful_modifies_trigger_event (prin:principal) (tag:string) (b:bytes) (tr:trace)
-  : Lemma (ensures (traceful_modifies (trigger_event prin tag b) tr) == empty)
-    [SMTPat (traceful_modifies (trigger_event prin tag b) tr)]
-  = reveal_opaque (`%trigger_event) (trigger_event)
-
-/// The core property --- if a trace (or traceful function) does not modify a given address,
+/// The core properties --- if a trace (or traceful function) does not modify a given address,
 /// the result of looking up the state at the start and end of that trace (traceful) is the same.
 
+val trace_concat_same_state_aux :
+  prin:principal -> sid:state_id ->
+  tr1:trace -> tr2:trace ->
+  Lemma
+  (requires ~((prin, sid) `mem` (trace_modifies tr2)))
+  (ensures get_state_aux prin sid tr1 == get_state_aux prin sid (tr1 <++> tr2))
+let trace_concat_same_state_aux prin sid tr1 tr2 =
+  let is_state_for prin sess_id e =
+    match e with
+    | SetState prin' sess_id' content -> prin = prin' && sess_id = sess_id'
+    | _ -> false
+  in
+  trace_modifies_spec tr2 prin sid;
+  introduce forall ts. ts `on_trace` tr2 ==> (~(is_state_for prin sid (get_entry_at tr2 ts)))
+  with introduce _ ==> _
+  with _. begin
+    match get_entry_at tr2 ts with
+    | SetState prin' sid' b -> ()
+    | _ -> ()
+  end;
+  trace_search_last_concat tr1 tr2 (is_state_for prin sid);
+  match trace_search_last tr1 (is_state_for prin sid) with
+  | None -> ()
+  | Some ts -> trace_concat_get_entry tr1 tr2 ts
 
-let rec trace_modifies_state_was_set (#label_t:Type) (prin:principal) (sid:state_id) (tr:trace_ label_t)
-  : Lemma
-    (ensures mem (prin, sid) (trace_modifies tr) <==> (exists b. state_was_set tr prin sid b))
-  = match tr with
-    | Nil -> ()
-    | Snoc hd e -> begin
-      trace_modifies_state_was_set prin sid hd;
-      if SetState? e && SetState?.prin e = prin && SetState?.sess_id e = sid
-      then begin
-        assert(state_was_set tr prin sid (SetState?.content e))
-      end
-      else ()
-    end
+val trace_grows_same_state_aux :
+  prin:principal -> sid:state_id ->
+  tr1:trace -> tr2:trace ->
+  Lemma
+  (requires tr1 <$ tr2 /\ ~((prin, sid) `mem` (trace_modifies (tr2 <--> tr1))))
+  (ensures (get_state_aux prin sid tr1) == (get_state_aux prin sid tr2))
+let trace_grows_same_state_aux prin sid tr1 tr2 =
+  trace_concat_same_state_aux prin sid tr1 (tr2 <--> tr1)
 
-let rec trace_concat_same_state_aux (prin:principal) (sid:state_id) (tr1 tr2:trace)
-  : Lemma
-    (requires ~((prin, sid) `mem` (trace_modifies tr2)))
-    (ensures (get_state_aux prin sid tr1) == (get_state_aux prin sid (tr1 <++> tr2)))
-  = match tr2 with
-    | Nil -> trace_concat_empty_trace tr1
-    | Snoc hd e -> begin
-      trace_concat_append_entry tr1 hd e;
-      trace_concat_same_state_aux prin sid tr1 hd;
-      assert((get_state_aux prin sid tr1) == (get_state_aux prin sid (tr1 <++> hd)));
-      match e with
-      | SetState prin' sid' _ -> assert(prin' <> prin || sid' <> sid)
-      | _ -> ()
-    end
+val traceful_unmodified_same_state_aux:
+  #a:Type ->
+  prin:principal -> sid:state_id ->
+  f:traceful a ->
+  tr_in:trace ->
+  Lemma
+  (requires ~((prin, sid) `mem` (traceful_modifies f tr_in)))
+  (ensures (
+    let (_, tr_out) = f tr_in in
+    get_state_aux prin sid tr_in == get_state_aux prin sid tr_out
+  ))
+let traceful_unmodified_same_state_aux prin sid f tr_in =
+  let (_, tr_out) = f tr_in in
+  trace_grows_same_state_aux prin sid tr_in tr_out
 
-let trace_grows_same_state_aux (prin:principal) (sid:state_id) (tr1 tr2:trace)
-  : Lemma
-    (requires tr1 <$ tr2 /\ ~((prin, sid) `mem` (trace_modifies (tr2 <--> tr1))))
-    (ensures (get_state_aux prin sid tr1) == (get_state_aux prin sid tr2))
-  = trace_concat_same_state_aux prin sid tr1 (tr2 <--> tr1)
 
 let trace_concat_same_state (prin:principal) (sid:state_id) (tr1 tr2:trace)
   : Lemma
@@ -276,7 +295,7 @@ let traceful_unmodified_same_state (#a:Type) (prin:principal) (sid:state_id) (f:
     ()
 
 /// TODO
-/// To be added to core?
+/// The next three functions seem like they belong in DY.Core.Trace.Manipulation
 val get_trace_same_trace (tr:trace)
   : Lemma
     (ensures (
@@ -296,21 +315,48 @@ val get_state_same_trace (prin:principal) (sid:state_id) (tr:trace)
     [SMTPat (get_state prin sid tr);]
 let get_state_same_trace prin sid tr = ()
 
+val set_state_get_state_aux:
+  prin:principal -> sess_id:state_id -> content:bytes ->
+  tr:trace ->
+  Lemma
+  (ensures (
+    let (_, tr_out) = set_state prin sess_id content tr in
+    get_state_aux prin sess_id tr_out == (Some content)
+  ))
+  [SMTPat (set_state prin sess_id content tr)]
+let set_state_get_state_aux prin sess_id content tr =
+  reveal_opaque (`%set_state) (set_state)
 
-let tmp7 (#a:Type) (prin:principal) (sid:state_id) (f:traceful a)
-  : Pure (traceful (option bytes & option bytes))
-    (requires (forall tr. ~((prin, sid) `mem` (traceful_modifies f tr))))
-    (ensures fun _ -> True)
+val get_state_get_state_aux:
+  prin:principal -> sess_id:state_id -> tr:trace ->
+  Lemma
+  (ensures (
+    let (content_opt, _) = get_state prin sess_id tr in
+    content_opt == get_state_aux prin sess_id tr
+  ))
+  [SMTPat (get_state prin sess_id tr)]
+let get_state_get_state_aux prin sess_id tr =
+  reveal_opaque (`%get_state) (get_state)
+
+/// TODO: Some simple testing of the analysis
+/// Should we put this in an example file? Remove it? Add some kind of test suite?
+
+let unmodified_test (prin:principal) (sid:state_id)
+  : traceful (option bytes & option bytes)
   = let* st_opt1 = get_state prin sid in
-    let* x = f in
+    let* new_rand = mk_rand NoUsage (DY.Core.Label.principal_label prin) 32 in
+    let* msg_ts = send_msg new_rand in
+    let* _ = trigger_event prin "test_event" (Literal (Seq.Base.empty)) in
+    let* _ = recv_msg msg_ts in
     let* st_opt2 = get_state prin sid in
     return (st_opt1, st_opt2)
 
-let tmp8 (#a:Type) (prin:principal) (sid:state_id) (f:traceful a) (tr_in:trace)
+#push-options "--z3rlimit 100"
+let unmodified_test_proof (prin:principal) (sid:state_id) (tr_in:trace)
   : Lemma
-    (requires (forall tr. ~((prin, sid) `mem` (traceful_modifies f tr))))
-    (ensures (
-      let ((st_opt1, st_opt2), tr_out) = test_traceful prin sid f tr_in in
-      st_opt1 == st_opt2
-    ))
-  = traceful_unmodified_same_state prin sid f tr_in
+    (let ((st_opt1, st_opt2), _) = unmodified_test prin sid tr_in in
+     st_opt1 == st_opt2
+    )
+  = assert(traceful_modifies (unmodified_test prin sid) tr_in == empty);
+    traceful_unmodified_same_state_aux prin sid (unmodified_test prin sid) tr_in;
+    ()
